Refactor and clean code

src/examples/interactive_tactic_entry.lean
@@ -1,9 +1,7 @@
-import interface
-open lean.parser
-open interactive
+import lean_gym.server
 
 -- set up server
-meta def server : json_server lean_server_request lean_server_response := {
+meta def  json_config : json_server lean_server_request lean_server_response := {
   get_line := io.get_line,    -- communicate via stdin
   put_line := io.put_str_ln,  -- communicate via stdout
   get_json := json_server.get_custom_json,   -- use custom format since faster
@@ -11,5 +9,6 @@ meta def server : json_server lean_server_request lean_server_response := {
 }
 
 theorem foo : 1=1 := begin
-run_interface_from_tactic server
+lean_gym.run_server_from_tactic json_config,
+refl
 end
