src/examples/main_entry.lean
@@ -1,7 +1,7 @@
-import interface
+import lean_gym.server
 
 -- set up server
-meta def server : json_server lean_server_request lean_server_response := {
+meta def json_config : json_server lean_server_request lean_server_response := {
   get_line := io.get_line,    -- communicate via stdin
   put_line := io.put_str_ln,  -- communicate via stdout
   get_json := json_server.get_custom_json,   -- use custom format since faster
@@ -9,5 +9,5 @@ meta def server : json_server lean_server_request lean_server_response := {
 }
 
 meta def main : io unit :=
-  run_interface_from_io server
+  lean_gym.run_server_from_io json_config
   
