src/examples/parser_entry.lean
@@ -1,9 +1,9 @@
-import interface
+import lean_gym.server
 open lean.parser
 open interactive
 
 -- set up server
-meta def server : json_server lean_server_request lean_server_response := {
+meta def json_config : json_server lean_server_request lean_server_response := {
   get_line := io.get_line,    -- communicate via stdin
   put_line := io.put_str_ln,  -- communicate via stdout
   get_json := json_server.get_custom_json,   -- use custom format since faster
@@ -11,9 +11,9 @@ meta def server : json_server lean_server_request lean_server_response := {
 }
 
 @[user_command]
-meta def run_interface_with_goal_cmd (meta_info : interactive.decl_meta_info) (_ : interactive.parse (tk "run_interface_with_goal")) : lean.parser unit :=
+meta def run_lean_gym_server_with_goal_cmd (meta_info : interactive.decl_meta_info) (_ : interactive.parse (tk "run_lean_gym_server_with_goal")) : lean.parser unit :=
 do goal <- interactive.types.texpr,
-  run_interface_from_parser server goal
+  lean_gym.run_server_from_parser json_config goal
 .
 
-run_interface_with_goal 1 + 1 = 2 . -- will succeed
+run_lean_gym_server_with_goal 1 + 1 = 2 . -- will succeed
