src/lean_gym/server.lean
@@ -1,0 +1,194 @@
+import lean_gym.interface_m
+import tools.serialization -- TODO: Serialize Lean's standard raw expression format
+import system.io
+
+-- read eval print loop
+namespace lean_gym
+
+meta def deserialize_expr (sexpr : string) : interface_m expr :=
+match (expr.deserialize sexpr) with
+| (sum.inl error_msg) := throw (interface_ex.user_input_exception ("Error parsing s-expression: " ++ error_msg))
+| (sum.inr h) := return h
+end
+
+meta def apply_tactic (t : tactic unit): interface_m tactic_state := do
+ts <- interface_m.get_current_tactic_state,
+catch (interface_m.run_tactic2 ts t) $ λ e, match e with
+| interface_ex.tactic_exception error := throw (interface_ex.apply_tactic_exception error)
+| e := throw e
+end
+
+meta def apply_tactic_request (ts : tactic_state) : lean_tactic -> interface_m tactic_state
+| (lean_tactic.apply sexpr) := do
+  h <- deserialize_expr sexpr,
+  apply_tactic (tactic.interactive.concat_tags (tactic.apply h))
+| (lean_tactic.cases sexpr) := do
+  h <- deserialize_expr sexpr,
+  apply_tactic (tactic.interactive.cases_core h [])
+| lean_tactic.intro := apply_tactic (tactic.interactive.propagate_tags (tactic.intro1 >> tactic.skip))
+| lean_tactic.split := apply_tactic (tactic.interactive.split)
+| lean_tactic.left := apply_tactic (tactic.interactive.left)
+| lean_tactic.right := apply_tactic (tactic.interactive.right)
+
+meta def mk_new_goal (ts0 : tactic_state) (goal : expr) : interface_m tactic_state := do
+interface_m.run_tactic2 ts0 $ (do
+  v <- tactic.mk_meta_var goal,
+  tactic.set_goals [v],
+  return ()
+)
+
+meta def change_goal (sexp : string) : interface_m unit := do
+  goal_expr <- deserialize_expr sexp,
+  ts0 <- interface_m.get_inital_tactic_state,
+  ts <- mk_new_goal ts0 goal_expr,
+  interface_m.reset_all_tactic_states ts
+
+meta def change_state : lean_state_control -> interface_m unit
+| (lean_state_control.jump_to_state state_index) := 
+  interface_m.set_tactic_state state_index
+| (lean_state_control.change_top_goal sexp) := 
+  change_goal sexp
+
+meta def state_info_str (st_ix : nat) : tactic string := do
+let s :=  "Proof state:",
+st ← tactic.read,
+let fmt := to_fmt st,
+fmt <- tactic.pp fmt,
+let s := s ++ "\n" ++ (to_string fmt),
+let s := s ++ "\n",
+let s := s ++ "\n" ++ "Current state index:",
+let s := s ++ "\n" ++ (to_string st_ix),
+let s := s ++ "\n",
+s1 <- (do 
+  let s1 := s ++ "\n" ++ "Local names:",
+  lctx ← tactic.local_context,
+  let ls := lctx.map (λ e, expr.representation.form_of_expr e),
+  let s1 :=  s1 ++ "\n" ++ (string.intercalate "\n" ls),
+  return s1
+) <|> (return s),
+return s1
+
+meta def get_state_info (ts : tactic_state) (ix : nat): interface_m string := do
+interface_m.run_tactic1 ts (state_info_str ix)
+
+meta def eval_user_request : lean_server_request → interface_m lean_server_response
+| (lean_server_request.apply_tactic tac) := catch (do
+    ts <- interface_m.get_current_tactic_state,
+    ts <- apply_tactic_request ts tac,
+    ix <- interface_m.register_tactic_state ts,
+    state_info <- get_state_info ts ix,
+    let msg := "Tactic succeeded:" ++ "\n" ++ state_info,
+    let result := lean_tactic_result.success msg,
+    let response := lean_server_response.apply_tactic result,
+    return response
+  ) $ λ e, match e with
+  | interface_ex.apply_tactic_exception fmt_opt := do
+    let msg := match fmt_opt with
+    | some fmt := "Tactic failed: " ++ (to_string (fmt ()))
+    | none := "Tactic failed: <no message>"
+    end,
+    let result := lean_tactic_result.failure msg,
+    let response := lean_server_response.apply_tactic result,
+    return response
+  | interface_ex.tactic_exception fmt_opt := do
+    let msg := match fmt_opt with
+    | some fmt := "Unable to apply tactic: " ++ (to_string (fmt ()))
+    | none := "Unable to apply tactic: <no message>"
+    end,
+    let result := lean_tactic_result.server_error msg,
+    let response := lean_server_response.apply_tactic result,
+    return response
+  | interface_ex.user_input_exception msg := do
+    let msg := "Unable to apply tactic: " ++ msg,
+    let result := lean_tactic_result.server_error msg,
+    let response := lean_server_response.apply_tactic result,
+    return response
+  | e := throw e
+  end
+| (lean_server_request.change_state state_control) := catch (do
+    change_state state_control,
+    ts <- interface_m.get_current_tactic_state,
+    ix <- interface_m.get_current_tactic_state_ix,
+    state_info <- get_state_info ts ix,
+    let msg := "state change succeeded:" ++ "\n" ++ state_info,
+    let result := lean_state_result.success msg,
+    let response := lean_server_response.change_state result,
+    return response
+  ) $ λ e, match e with
+  | interface_ex.tactic_exception fmt_opt := do
+    let msg := match fmt_opt with
+    | some fmt := "State change failed: " ++ (to_string (fmt ()))
+    | none := "State change failed: <no message>"
+    end,
+    let result := lean_state_result.server_error msg,
+    let response := lean_server_response.change_state result,
+    return response
+  | interface_ex.user_input_exception msg := do
+    let msg := "State change failed: " ++ msg,
+    let result := lean_state_result.server_error msg,
+    let response := lean_server_response.change_state result,
+    return response
+  | e := throw e
+  end
+
+meta def server_loop : interface_m unit := do
+response <- catch (do 
+  -- TODO: Might want to split into errors that are parsing errors (json type things) and ones that are bugs on my end
+  request <- interface_m.read_io_request,
+  eval_user_request request
+) (λ e, 
+  match e with
+  | interface_ex.tactic_exception fmt_opt := do
+    let msg := match fmt_opt with
+    | some fmt := "Unexpected error processing request: " ++ (to_string (fmt ()))
+    | none := "Unexpected error processing request: <no message>"
+    end,
+    let response := lean_server_response.error msg,
+    return response
+  | e := throw e 
+  end
+),
+interface_m.write_io_response response,
+server_loop
+
+-- commands for running the interface
+-- TODO: maybe it is better not to have the initial tactic state inside the config
+--       so that the config can be made ahead of time
+meta def run_server_from_tactic (server : json_server lean_server_request lean_server_response) : tactic (except interface_ex unit) := do
+  ts <- get_state,
+  let config : interface_config := {
+    server := server,
+    ps := none,
+    initial_ts := ts
+  },
+  -- it is very important that we do something with `server_loop.run config`
+  -- (like return it) otherwise it won't be executed
+  return $ server_loop.run config
+  
+meta def get_parser_state : lean.parser lean.parser_state :=
+λ ps, interaction_monad.result.success ps ps
+
+meta def tactic_state_at_goal (goal : pexpr) : lean.parser tactic_state :=
+lean.parser.of_tactic $ do
+  e <- tactic.to_expr goal,
+  v <- tactic.mk_meta_var e,
+  tactic.set_goals [v],
+  ts <- get_state,
+  return ts
+
+meta def run_server_from_parser (server : json_server lean_server_request lean_server_response) (goal : pexpr) : lean.parser unit := do
+  ps <- get_parser_state,
+  ts <- tactic_state_at_goal goal,
+  let config : interface_config := {
+    server := server,
+    ps := ps,
+    initial_ts := ts
+  },
+  let ts := server_loop.run config,
+  return ()
+
+meta def run_server_from_io (server : json_server lean_server_request lean_server_response): io unit := do
+  io.run_tactic (run_server_from_tactic server),
+  return ()
+
+end lean_gym
